renaming

Higher_Order_Tests.thy
@@ -3,64 +3,64 @@ imports
   Hint_Unification
 begin
 
-ML_file \<open>Test.ML\<close>
+ML_file ‹Test.ML›
 
-ML\<open>
+ML‹
   open Test
   open Utils
-  val hint_unif = HO_Pat_Hint_Unif.h_unify
+  val hint_unif = HO_Pat_Hint_Unif.hint_unify
   fun std_unif ctxt ts env = (Pattern.unify ctxt ts env,@{thm Pure.reflexive})
-  val ctxt = Context.the_generic_context\<close>
+  val ctxt = Context.the_generic_context›
 
-setup\<open>term_pat_setup\<close>
+setup‹term_pat_setup›
 declare [[log_level=500]]
 
 (* Symmetry *)
-ML\<open>test_group symmetry std_unif "Free/Var" free_var_gen\<close>
-ML\<open>test_group symmetry hint_unif "Free/Var" free_var_gen\<close>
+ML‹test_group symmetry std_unif "Free/Var" free_var_gen›
+ML‹test_group symmetry hint_unif "Free/Var" free_var_gen›
 
 (* Correct Environment is returned *)
-ML\<open>test_group sigma_unifies std_unif "Free/Var" free_var_gen\<close>
-ML\<open>test_group sigma_unifies hint_unif "Free/Var" free_var_gen\<close>
+ML‹test_group sigma_unifies std_unif "Free/Var" free_var_gen›
+ML‹test_group sigma_unifies hint_unif "Free/Var" free_var_gen›
 
-ML\<open>test_group sigma_unifies_var_term std_unif "Free/Var" free_var_gen\<close>
-ML\<open>test_group sigma_unifies_var_term hint_unif "Free/Var" free_var_gen\<close>
+ML‹test_group sigma_unifies_var_term std_unif "Free/Var" free_var_gen›
+ML‹test_group sigma_unifies_var_term hint_unif "Free/Var" free_var_gen›
 
-ML\<open>test_group sigma_unifies_vars_replaced std_unif "Free/Var" free_var_gen\<close>
-ML\<open>test_group sigma_unifies_vars_replaced hint_unif "Free/Var" free_var_gen\<close>
+ML‹test_group sigma_unifies_vars_replaced std_unif "Free/Var" free_var_gen›
+ML‹test_group sigma_unifies_vars_replaced hint_unif "Free/Var" free_var_gen›
 
 (** non-unifiability tests **)
 (* Occurs check stops unification *)
-ML\<open>test_group occurs_check std_unif "Var only" var_gen\<close>
-ML\<open>test_group occurs_check hint_unif "Var only" var_gen\<close>
+ML‹test_group occurs_check std_unif "Var only" var_gen›
+ML‹test_group occurs_check hint_unif "Var only" var_gen›
 
 (** manual tests with Var/Free and TVar/TFree **)
 (* should unify, using std_unif *)
-ML\<open>list_pos (ctxt ()) std_unif "Var/Free, TVar/TFree combinations unify"
+ML‹list_pos (ctxt ()) std_unif "Var/Free, TVar/TFree combinations unify"
   [(Var(("A",0),TVar(("'a",0),[])),Free("A",TFree("'a",[]))),
    (Var(("A",0),TVar(("'a",0),[])),Var(("A",0),TFree("'a",[]))),
    (Var(("A",0),TVar(("'a",0),[])),Var(("B",0),TVar(("'a",0),[]))),
    (Var(("A",0),TVar(("'a",0),[])),Var(("A",0),TVar(("'b",0),[]))),
    (Var(("A",0),TFree("'a",[])),Free("A",TVar(("'a",0),[]))),
-   (Free("A",TFree("'a",[])),Free("A",TVar(("'a",0),[])))]\<close>
+   (Free("A",TFree("'a",[])),Free("A",TVar(("'a",0),[])))]›
 
 (* should unify, using hint_unif *)
-ML\<open>list_pos (ctxt ()) hint_unif "Var/Free, TVar/TFree combinations unify"
+ML‹list_pos (ctxt ()) hint_unif "Var/Free, TVar/TFree combinations unify"
   [(Var(("A",0),TVar(("'a",0),[])),Free("A",TFree("'a",[]))),
    (Var(("A",0),TVar(("'a",0),[])),Var(("A",0),TFree("'a",[]))),
    (Var(("A",0),TVar(("'a",0),[])),Var(("B",0),TVar(("'a",0),[]))),
    (Var(("A",0),TVar(("'a",0),[])),Var(("A",0),TVar(("'b",0),[]))),
    (Var(("A",0),TFree("'a",[])),Free("A",TVar(("'a",0),[]))),
-   (Free("A",TFree("'a",[])),Free("A",TVar(("'a",0),[])))]\<close>
+   (Free("A",TFree("'a",[])),Free("A",TVar(("'a",0),[])))]›
 
 (* should not unify, using std_unif *)
-ML\<open>list_neg (ctxt ()) std_unif "Different Free/TFree fails"
+ML‹list_neg (ctxt ()) std_unif "Different Free/TFree fails"
   [(Free("A",TFree("'a",[])),Free("A",TFree("'b",[]))),
-   (Free("A",TFree("'a",[])),Free("B",TFree("'a",[])))]\<close>
+   (Free("A",TFree("'a",[])),Free("B",TFree("'a",[])))]›
 (* should not unify, using hint_unif *)
-ML\<open>list_neg (ctxt ()) hint_unif "Different Free/TFree fails"
+ML‹list_neg (ctxt ()) hint_unif "Different Free/TFree fails"
   [(Free("A",TFree("'a",[])),Free("A",TFree("'b",[]))),
-   (Free("A",TFree("'a",[])),Free("B",TFree("'a",[])))]\<close>
+   (Free("A",TFree("'a",[])),Free("B",TFree("'a",[])))]›
 
 
 
@@ -69,177 +69,177 @@ ML\<open>list_neg (ctxt ()) hint_unif "Different Free/TFree fails"
 
 (* non-recursive hint tests *)
 (*add_zero*)
-ML\<open>
+ML‹
   val (t1,t2) = (@{term_pat "5::nat"}, @{term_pat "?b + 0 ::nat"});
-  single_neg (ctxt ()) hint_unif "add_zero without hint" (t1,t2)\<close>
-lemma add_zero [hints]: "Y \<equiv> Z \<Longrightarrow>  X \<equiv> (0::nat) \<Longrightarrow> Y + X \<equiv> Z"
+  single_neg (ctxt ()) hint_unif "add_zero without hint" (t1,t2)›
+lemma add_zero [hints]: "Y ≡ Z ⟹  X ≡ (0::nat) ⟹ Y + X ≡ Z"
   by simp
-ML\<open>single_pos (ctxt ()) hint_unif "add_zero with hint" (t1,t2)\<close>
+ML‹single_pos (ctxt ()) hint_unif "add_zero with hint" (t1,t2)›
 
 (*mult_one*)
-ML\<open>
+ML‹
   val (t1,t2) = (@{term_pat "1::nat"},@{term_pat "?a * ?b ::nat"});
-  single_neg (ctxt ()) hint_unif "mult_one without hint" (t1,t2)\<close>
-lemma mult_one [hints]: "X \<equiv> 1 \<Longrightarrow> Y \<equiv> 1 \<Longrightarrow> X * Y \<equiv> (1::nat)"
+  single_neg (ctxt ()) hint_unif "mult_one without hint" (t1,t2)›
+lemma mult_one [hints]: "X ≡ 1 ⟹ Y ≡ 1 ⟹ X * Y ≡ (1::nat)"
   by simp
-ML\<open>single_pos (ctxt ()) hint_unif "mult_one with hint" (t1,t2)\<close>
+ML‹single_pos (ctxt ()) hint_unif "mult_one with hint" (t1,t2)›
 
 (*id_eq*)
-ML\<open>
+ML‹
   val (t1,t2) = (@{term_pat "5::nat"},@{term_pat "id ?a ::nat"});
-  single_neg (ctxt ()) hint_unif "id_eq without hint" (t1,t2)\<close>
-lemma ID_EQ [hints]: "X \<equiv> Y \<Longrightarrow> id X \<equiv> Y"
+  single_neg (ctxt ()) hint_unif "id_eq without hint" (t1,t2)›
+lemma ID_EQ [hints]: "X ≡ Y ⟹ id X ≡ Y"
   by simp
-ML\<open>single_pos (ctxt ()) hint_unif "id_eq with hint" (t1,t2)\<close>
+ML‹single_pos (ctxt ()) hint_unif "id_eq with hint" (t1,t2)›
 
 (*Suc 2 = 3*)
-ML\<open>
+ML‹
   val (t1,t2) = (@{term_pat "Suc ?x ::nat"},@{term_pat "3::nat"});
-  single_neg (ctxt ()) hint_unif "Suc ?x = 3 without hint" (t1,t2)\<close>
-lemma suc2 [hints]: "X \<equiv> 2 \<Longrightarrow> Suc X \<equiv> 3"
+  single_neg (ctxt ()) hint_unif "Suc ?x = 3 without hint" (t1,t2)›
+lemma suc2 [hints]: "X ≡ 2 ⟹ Suc X ≡ 3"
   by linarith
-ML\<open>single_pos (ctxt ()) hint_unif "Suc ?x = 3 with hint" (t1,t2)\<close>
+ML‹single_pos (ctxt ()) hint_unif "Suc ?x = 3 with hint" (t1,t2)›
 
 (*Suc x = 4, multiple matching hints, first one doesn't unify*)
-definition x_def: "x\<equiv>3::nat"
-ML\<open>
+definition x_def: "x≡3::nat"
+ML‹
   val (t1,t2) =(@{term_pat "Suc x ::nat"},@{term_pat "4::nat"});
-  single_neg (ctxt ()) hint_unif "Suc x = 4 without hint" (t1,t2)\<close>
-lemma suc_x_4 [hints]: "Suc x \<equiv> 4"
+  single_neg (ctxt ()) hint_unif "Suc x = 4 without hint" (t1,t2)›
+lemma suc_x_4 [hints]: "Suc x ≡ 4"
   by (simp add:x_def)
-lemma suc3 [hints]: "X \<equiv> 3 \<Longrightarrow> Suc X \<equiv> 4"
+lemma suc3 [hints]: "X ≡ 3 ⟹ Suc X ≡ 4"
   by linarith
-ML\<open>single_pos (ctxt ()) hint_unif "Suc x = 4 with multiple matching hints, only second one solves"
-  (t1,t2)\<close>
+ML‹single_pos (ctxt ()) hint_unif "Suc x = 4 with multiple matching hints, only second one solves"
+  (t1,t2)›
 
 (* recursive hint tests *)
 
 (*Suc (Suc 0) = 2*)
-ML\<open>
+ML‹
   val (t1,t2) = (@{term_pat "Suc (Suc ?X) ::nat"},@{term_pat "2::nat"});
-  single_neg (ctxt ()) hint_unif "Suc ?x = 3 without hint" (t1,t2)\<close>
-lemma suc0 [hints]: "X \<equiv> 0 \<Longrightarrow> Suc X \<equiv> 1"
+  single_neg (ctxt ()) hint_unif "Suc ?x = 3 without hint" (t1,t2)›
+lemma suc0 [hints]: "X ≡ 0 ⟹ Suc X ≡ 1"
   by linarith
-lemma suc1 [hints]: "X \<equiv> 1 \<Longrightarrow> Suc X \<equiv> 2"
+lemma suc1 [hints]: "X ≡ 1 ⟹ Suc X ≡ 2"
   by linarith
-ML\<open>single_pos (ctxt ()) hint_unif "Suc ?x = 3 with hints" (t1,t2)\<close>
+ML‹single_pos (ctxt ()) hint_unif "Suc ?x = 3 with hints" (t1,t2)›
 
 
-consts f :: "nat \<Rightarrow> nat" g :: "nat \<Rightarrow> nat" h :: "nat \<Rightarrow> nat"
+consts f :: "nat ⇒ nat" g :: "nat ⇒ nat" h :: "nat ⇒ nat"
        a :: nat b :: nat y::nat
 
-lemma [hints] : "X \<equiv> f (g 0) \<Longrightarrow> Y \<equiv> g (f 0) \<Longrightarrow> f (g X) \<equiv> g (f Y)"
+lemma [hints] : "X ≡ f (g 0) ⟹ Y ≡ g (f 0) ⟹ f (g X) ≡ g (f Y)"
   sorry
-ML\<open>
+ML‹
   val (t1,t2) = (@{term_pat "f (g (f (g 0))) ::nat"}, @{term_pat "g (f (g (f 0))) ::nat"});
-  single_pos (ctxt ()) hint_unif "" (t1,t2);\<close>
+  single_pos (ctxt ()) hint_unif "" (t1,t2);›
 
 (*same hint but with premises switched*)
-consts f2 :: "nat \<Rightarrow> nat" g2 :: "nat \<Rightarrow> nat"
-lemma [hints] : "Y \<equiv> g2 (f2 0) \<Longrightarrow> X \<equiv> f2 (g2 0) \<Longrightarrow> f2 (g2 X) \<equiv> g2 (f2 Y)"
+consts f2 :: "nat ⇒ nat" g2 :: "nat ⇒ nat"
+lemma [hints] : "Y ≡ g2 (f2 0) ⟹ X ≡ f2 (g2 0) ⟹ f2 (g2 X) ≡ g2 (f2 Y)"
   sorry
-ML\<open>
+ML‹
   val (t1,t2) = (@{term_pat "f2 (g2 (f2 (g2 0))) ::nat"}, @{term_pat "g2 (f2 (g2 (f2 0))) ::nat"});
-  single_pos (ctxt ()) hint_unif "" (t1,t2);\<close>
+  single_pos (ctxt ()) hint_unif "" (t1,t2);›
 
-lemma [hints]: "Y \<equiv> f X \<Longrightarrow> X \<equiv> f (g 0) \<Longrightarrow>  f (g X) \<equiv> g (f Y)"
+lemma [hints]: "Y ≡ f X ⟹ X ≡ f (g 0) ⟹  f (g X) ≡ g (f Y)"
   sorry
-ML\<open>
+ML‹
   val (t1,t2) = (@{term_pat "f (g (f (g 0))) ::nat"}, @{term_pat "g (f (f (f (g 0)))) ::nat"});
-  single_pos (ctxt ()) hint_unif "" (t1,t2);\<close>
+  single_pos (ctxt ()) hint_unif "" (t1,t2);›
 
 (*same hint but with premises switched*)
-lemma [hints]: "X \<equiv> f2 (g2 0) \<Longrightarrow> Y \<equiv> f2 X \<Longrightarrow>  f2 (g2 X) \<equiv> g2 (f2 Y)"
+lemma [hints]: "X ≡ f2 (g2 0) ⟹ Y ≡ f2 X ⟹  f2 (g2 X) ≡ g2 (f2 Y)"
   sorry
-ML\<open>
+ML‹
   val (t1,t2) = (@{term_pat "f2 (g2 (f2 (g2 0))) ::nat"}, @{term_pat "g2 (f2 (f2 (f2 (g2 0)))) ::nat"});
-  single_pos (ctxt ()) hint_unif "" (t1,t2);\<close>
+  single_pos (ctxt ()) hint_unif "" (t1,t2);›
 
 (*recursive calls with encapsulated hints*)
-lemma [hints]:"X \<equiv> f \<Longrightarrow> X a \<equiv> X b"
+lemma [hints]:"X ≡ f ⟹ X a ≡ X b"
   sorry
 
-lemma [hints]:"X \<equiv> Y \<Longrightarrow> h (g X) \<equiv> g (h Y)"
+lemma [hints]:"X ≡ Y ⟹ h (g X) ≡ g (h Y)"
   sorry
 
-ML\<open>
+ML‹
   val (t1,t2) = (@{term_pat "h (g (f a))"},@{term_pat "g (h (f b))"});
-  single_pos (ctxt ()) hint_unif "" (t1,t2);\<close>
+  single_pos (ctxt ()) hint_unif "" (t1,t2);›
 
-ML\<open>
+ML‹
   val (t1,t2) = (@{term_pat "id (id 2) ::nat"}, @{term_pat "Suc ?x ::nat"});
-  single_pos (ctxt ()) hint_unif "" (t1,t2);\<close>
+  single_pos (ctxt ()) hint_unif "" (t1,t2);›
 
-consts r :: "nat \<Rightarrow> nat \<Rightarrow> nat" t :: "nat \<Rightarrow> nat"
+consts r :: "nat ⇒ nat ⇒ nat" t :: "nat ⇒ nat"
 
 (*recursive calls with alternating hints*)
-lemma [hints]:"X \<equiv> Y \<Longrightarrow> f X \<equiv> g Y"
+lemma [hints]:"X ≡ Y ⟹ f X ≡ g Y"
   sorry
 
-lemma [hints]:"X \<equiv> Y \<Longrightarrow> f2 X \<equiv> g2 Y"
+lemma [hints]:"X ≡ Y ⟹ f2 X ≡ g2 Y"
   sorry
 
-ML\<open>
+ML‹
   val (t1,t2) = (@{term_pat "f2 (f (g 0)) ::nat"}, @{term_pat "g2 (f (g 0)) ::nat"});
-  single_pos (ctxt ()) hint_unif "" (t1,t2);\<close>
+  single_pos (ctxt ()) hint_unif "" (t1,t2);›
 
 (*premise order: case where Xi depends on Xj with j>i cannot unify*)
 consts l::nat m::nat 
 
-lemma h1[hints]: "X1 \<equiv> X2 l \<Longrightarrow> X2 \<equiv> f \<Longrightarrow> X1 \<equiv> f m"
+lemma h1[hints]: "X1 ≡ X2 l ⟹ X2 ≡ f ⟹ X1 ≡ f m"
   sorry
 
-ML\<open>
+ML‹
   val (t1,t2) = (@{term_pat "f l ::nat"}, @{term_pat "f m ::nat"});
-  single_neg (ctxt ()) hint_unif "" (t1,t2);\<close>
+  single_neg (ctxt ()) hint_unif "" (t1,t2);›
 
 
 (*Higher-order-exclusive tests*)
-ML\<open>
-  val (t1,t2) = (@{term_pat "\<lambda>x. f x"},@{term_pat "\<lambda>x. f x"});
-  trace_test_result (ctxt()) (t1,t2) hint_unif\<close>
+ML‹
+  val (t1,t2) = (@{term_pat "λx. f x"},@{term_pat "λx. f x"});
+  trace_test_result (ctxt()) (t1,t2) hint_unif›
 
-ML\<open>
-  val (t1,t2) = (@{term_pat "\<lambda>x. \<lambda>y. (x::nat)"},@{term_pat "\<lambda>y. \<lambda>x. y"});
-  trace_test_result (ctxt()) (t1,t2) hint_unif\<close>
+ML‹
+  val (t1,t2) = (@{term_pat "λx. λy. (x::nat)"},@{term_pat "λy. λx. y"});
+  trace_test_result (ctxt()) (t1,t2) hint_unif›
 
-ML\<open>
-  val (t1,t2) = (@{term_pat "\<lambda>x. r x ?Y"},@{term_pat "\<lambda>x. r x ?Y"});
-  trace_test_result (ctxt()) (t1,t2) hint_unif\<close>
+ML‹
+  val (t1,t2) = (@{term_pat "λx. r x ?Y"},@{term_pat "λx. r x ?Y"});
+  trace_test_result (ctxt()) (t1,t2) hint_unif›
 
-lemma [hints]:"X\<equiv>(0::nat) \<Longrightarrow> Y\<equiv>Z \<Longrightarrow> X + Y \<equiv>Z"
+lemma [hints]:"X≡(0::nat) ⟹ Y≡Z ⟹ X + Y ≡Z"
 by linarith
-ML\<open>
-  val (t1,t2) = (@{term_pat "\<lambda>x. (\<lambda>y. 0 + 1::nat)"},@{term_pat "\<lambda>x. (\<lambda>y. 1::nat)"});
-  trace_test_result (ctxt()) (t1,t2) hint_unif\<close>
+ML‹
+  val (t1,t2) = (@{term_pat "λx. (λy. 0 + 1::nat)"},@{term_pat "λx. (λy. 1::nat)"});
+  trace_test_result (ctxt()) (t1,t2) hint_unif›
 
-ML\<open>
-  val (t1,t2) = (@{term_pat "(\<lambda>x. 0 + Z + x::nat)"},@{term_pat "(\<lambda>x. Z + x::nat)"});
-  trace_test_result (ctxt()) (t1,t2) hint_unif\<close>
+ML‹
+  val (t1,t2) = (@{term_pat "(λx. 0 + Z + x::nat)"},@{term_pat "(λx. Z + x::nat)"});
+  trace_test_result (ctxt()) (t1,t2) hint_unif›
 
-ML\<open>
-  val (t1,t2) = (@{term_pat "\<lambda>x. (\<lambda>y. 0 + Suc ?x::nat)"},@{term_pat "\<lambda>x. (\<lambda>y. 3::nat)"});
-  trace_test_result (ctxt()) (t1,t2) hint_unif\<close>
+ML‹
+  val (t1,t2) = (@{term_pat "λx. (λy. 0 + Suc ?x::nat)"},@{term_pat "λx. (λy. 3::nat)"});
+  trace_test_result (ctxt()) (t1,t2) hint_unif›
 
 consts
-  A :: "(nat \<Rightarrow> nat) \<times> nat \<Rightarrow> nat"
-  B :: "nat \<times> nat \<Rightarrow> nat"
+  A :: "(nat ⇒ nat) × nat ⇒ nat"
+  B :: "nat × nat ⇒ nat"
   C :: "nat"
 
-ML\<open>
-  val (t1,t2) = (@{term_pat "\<lambda>u. B (?x,u)"},@{term_pat "\<lambda>v. B (C,v)"});
-  trace_test_result (ctxt()) (t1,t2) hint_unif\<close>
+ML‹
+  val (t1,t2) = (@{term_pat "λu. B (?x,u)"},@{term_pat "λv. B (C,v)"});
+  trace_test_result (ctxt()) (t1,t2) hint_unif›
 
-ML\<open>
-  val (t1,t2) = (@{term_pat "A (\<lambda>u. B (?x,u),C)"},@{term_pat "A (\<lambda>v. B (C,v),?y)"});
-  trace_test_result (ctxt()) (t1,t2) hint_unif\<close>
+ML‹
+  val (t1,t2) = (@{term_pat "A (λu. B (?x,u),C)"},@{term_pat "A (λv. B (C,v),?y)"});
+  trace_test_result (ctxt()) (t1,t2) hint_unif›
 
-ML\<open>
-  val (t1,t2) = (@{term_pat "A (\<lambda>u. B (?x,C), C)"},@{term_pat "id (A (\<lambda>u. ?y, C+0))"});
-  trace_test_result (ctxt()) (t1,t2) hint_unif\<close>
+ML‹
+  val (t1,t2) = (@{term_pat "A (λu. B (?x,C), C)"},@{term_pat "id (A (λu. ?y, C+0))"});
+  trace_test_result (ctxt()) (t1,t2) hint_unif›
 
 (*Bound case not working yet*)
-ML\<open>
-  val (t1,t2) = (@{term_pat "\<lambda>x. (\<lambda>x. 0+x::nat)"},@{term_pat "\<lambda>x. (\<lambda>x. x::nat)"});\<close>
+ML‹
+  val (t1,t2) = (@{term_pat "λx. (λx. 0+x::nat)"},@{term_pat "λx. (λx. x::nat)"});›
 
 end
